lawyer/nonblocking/om_wfree_inst.v
@@ -59,8 +59,14 @@ Proof using.
 Abort. 
 
 
-(* TODO: relax to non-trivial degrees *)
-(* TODO: support LATs *)
+(** Lawyer representation of wait-freedom of a "first-order" function `m`.
+    Consists of two specs: model-based and physical-only.
+    Neither of them restricts the arguments that `m` is called with.
+    With that, the model-based spec implies that `m` must safely terminate with any argument while preserving physical and model interpretation, as well as invariants.
+    Physical-only spec requires that physical interpretation and invariants are preserved, while allowing `m` to get stuck (however, since it satisfies the model-based spec, it won't actually get stuck).
+    Both specifications rely on the module invariant `wfs_mod_inv`.
+    It is crucial that this invariant doesn't involve any model resources (compare e.g. Σ restrictions for the invariant and the model-based spec).
+    That's because it has to be preserved when either of the specs is used. *)
 Record WaitFreeSpec (m: val) := {
   wfs_is_init_st: cfg heap_lang -> Prop;
   (** for wait-free modules, we expect that invariant doesn't contain OM resources *)
@@ -70,14 +76,82 @@ Record WaitFreeSpec (m: val) := {
   wfs_init_mod `{heap1GS Σ, invGS_gen HasNoLc Σ}:
     forall c (INIT: wfs_is_init_st c),
       ⊢ hl_phys_init_resource c ={⊤}=∗ wfs_mod_inv;
+
+  
   wfs_F: nat;
+  (* TODO: relax to non-trivial degrees? *)
   wfs_spec:
   forall {M} {EM: ExecutionModel heap_lang M} {Σ} {OHE: OM_HL_Env OP_HL_WF EM Σ},
     (let _: heap1GS Σ := iem_phys HeapLangEM EM in wfs_mod_inv) ⊢
     wait_free_method m d_wfr0 wfs_F;
 
-  (* TODO: derive it from wfs_spec *)
   wfs_safety_spec:
     ∀ {Σ : gFunctors} `{heap1GS Σ, invGS_gen HasNoLc Σ},
       wfs_mod_inv ⊢ interp m;
+}.
+
+
+Definition ho_arg_restr {M} {EM: ExecutionModel heap_lang M} {Σ} {OHE: OM_HL_Env OP_HL_WF EM Σ}
+  (f: val) (P: val -> Prop) (F: nat) (fa: val) : iProp Σ :=
+  ∃ a, ⌜ fa = PairV f a /\ P a ⌝ ∗ wait_free_method f d_wfr0 F. 
+
+Record WaitFreeSpecHO (m: val) (P: val -> Prop) := {
+  wfsho_is_init_st: cfg heap_lang -> Prop;
+  (** for wait-free modules, we expect that invariant doesn't contain OM resources *)
+  wfsho_mod_inv {Σ} {hG: heap1GS Σ} {iG: invGS_gen HasNoLc Σ}: iProp Σ;
+  wfsho_mod_inv_Pers `{heap1GS Σ, invGS_gen HasNoLc Σ} ::
+    Persistent wfsho_mod_inv;
+  wfsho_init_mod `{heap1GS Σ, invGS_gen HasNoLc Σ}:
+    forall c (INIT: wfsho_is_init_st c),
+      ⊢ hl_phys_init_resource c ={⊤}=∗ wfsho_mod_inv;
+
+
+  (** The amount of fuel consumed by higher-order function is determined by:
+      - amount of fuel consumed by its function argument
+      - the actual argument (e.g. length of the list) *)
+  wfsho_F_fun: nat -> val -> nat;
+  (** We assume our higher-order function `m` in the uncurried form, e.g.
+        list_map x = let '(f, l) = x in ...
+      Then, we consider the calls of form `m (f, a)`, where `f` is an arbitrary (first-order) function and `a` fits the additional restriction (e.g. being a list).
+      For `f`, we assume that the first-order wait-free Trillium spec holds.
+      With that, if enough fuel is provided, the call must safely terminate. *)
+  wfsho_spec:
+  forall {M} {EM: ExecutionModel heap_lang M} {Σ} {OHE: OM_HL_Env OP_HL_WF EM Σ}
+    (f: val) (F_inner: nat),
+    (let _: heap1GS Σ := iem_phys HeapLangEM EM in wfsho_mod_inv) ⊢
+    wait_free_method_gen m d_wfr0 (wfsho_F_fun F_inner)
+      (ho_arg_restr f P F_inner) (fun _ => emp);
+
+  (** Contrary to the Lawyer spec above, physical-only spec doesn't place any restrictions on the argument (besides satisfying LR for values).
+      That's because in an arbitrary client, `m` can be called with any argument before the "target" call (considered by the adequacy theorem) happens.
+      We expect that `m` will get stuck if the argument doesn't fit the form defined in ho_arg_restr (e.g. when an argument to list_map is not a pair of some function and a list). 
+   *)
+  wfsho_safety_spec:
+    ∀ {Σ : gFunctors} `{heap1GS Σ, invGS_gen HasNoLc Σ},
+      wfsho_mod_inv ⊢ interp m;
+}. 
+
+
+(** WIP; should become a generalization of both specs above *)
+Record WaitFreeSpecGen (m: val)
+  (WF_P WF_Q: forall {M} {EM: ExecutionModel heap_lang M} {Σ} {OHE: OM_HL_Env OP_HL_WF EM Σ}, val -> iProp Σ)
+  := {
+  (* wfs_is_init_st: cfg heap_lang -> Prop; *)
+  (* (** for wait-free modules, we expect that invariant doesn't contain OM resources *) *)
+  (* wfs_mod_inv {Σ} {hG: heap1GS Σ} {iG: invGS_gen HasNoLc Σ}: iProp Σ; *)
+  (* wfs_mod_inv_Pers `{heap1GS Σ, invGS_gen HasNoLc Σ} :: *)
+  (*   Persistent wfs_mod_inv; *)
+  (* wfs_init_mod `{heap1GS Σ, invGS_gen HasNoLc Σ}: *)
+  (*   forall c (INIT: wfs_is_init_st c), *)
+  (*     ⊢ hl_phys_init_resource c ={⊤}=∗ wfs_mod_inv; *)
+  (* wfs_F: nat; *)
+  (* wfs_spec: *)
+  (* forall {M} {EM: ExecutionModel heap_lang M} {Σ} {OHE: OM_HL_Env OP_HL_WF EM Σ}, *)
+  (*   (let _: heap1GS Σ := iem_phys HeapLangEM EM in wfs_mod_inv) ⊢ *)
+  (*   wait_free_method m d_wfr0 wfs_F; *)
+
+  (* (* TODO: derive it from wfs_spec *) *)
+  (* wfs_safety_spec: *)
+  (*   ∀ {Σ : gFunctors} `{heap1GS Σ, invGS_gen HasNoLc Σ}, *)
+  (*     wfs_mod_inv ⊢ interp m; *)    
 }. 
