lawyer/nonblocking/wait_free_spec_defs.v
@@ -17,14 +17,15 @@ Definition wait_free_method
       App m a @ τ
     {{{ v, RET v; th_phase_frag τ π q }}}. 
 
+
 (* TODO: unify *)
 Definition wait_free_method_gen
   {M} {EM: ExecutionModel heap_lang M} {Σ} `{OP: OP_HL DegO LvlO LIM}
   {OHE: OM_HL_Env OP EM Σ}
-  (m: val) (d: DegO) (F: nat) (P Q: val -> Prop)
+  (m: val) (d: DegO) (F: val -> nat) (P Q: val -> iProp Σ)
   : iProp Σ :=
   ∀ τ π q (a: val), 
-    {{{ cp_mul π d F ∗ th_phase_frag τ π q ∗ ⌜ P a ⌝ }}}
+    {{{ cp_mul π d (F a) ∗ th_phase_frag τ π q ∗ P a }}}
       App m a @ τ
-    {{{ v, RET v; th_phase_frag τ π q ∗ ⌜ Q v ⌝ }}}. 
+    {{{ v, RET v; th_phase_frag τ π q ∗ Q v }}}. 
   
